PartialCombinatoryAlgebras/CombinatoryAlgebra.lean
@@ -1,0 +1,51 @@
+import Mathlib.Data.Part
+import PartialCombinatoryAlgebras.Basic
+
+/-- A (total) combinatory structure on a set `A`. -/
+class CA (A : Type*) extends HasDot A where
+  K : A
+  S : A
+  eq_K : ∀ {a b : A}, K ⬝ a ⬝ b = a
+  eq_S : ∀ (a b c : A), S ⬝ a ⬝ b ⬝ c = (a ⬝ c) ⬝ (b ⬝ c)
+
+attribute [simp] PCA.eq_K
+attribute [simp] PCA.eq_S
+
+/-- Missing from `Part` -/
+@[simps]
+def Part.map₂ {α β γ : Type*} (f : α → β → γ) (u : Part α) (v : Part β) : Part γ :=
+  ⟨u.Dom ∧ v.Dom, fun p => f (u.get (And.left p)) (v.get (And.right p))⟩
+
+@[simp]
+lemma Part.eq_map₂_some {α β γ : Type*} (f : α → β → γ) (a : α) (b : β) :
+  Part.map₂ f (.some a) (.some b) = .some (f a b) := by
+  ext c
+  simp [map₂]
+  constructor <;> apply Eq.symm
+
+namespace CA
+
+  /-- A total application induces a partial application -/
+  @[reducible]
+  instance partialApp {A : Type} [d : HasDot A] : PartialApplication A where
+    app := Part.map₂ d.dot
+
+  lemma eq_app {A : Type} [HasDot A] {u v : Part A} (hu : u ⇓) (hv : v ⇓):
+    u ⬝ v = .some (u.get hu ⬝ v.get hv) := by
+    nth_rewrite 1 [←Part.some_get hu]
+    nth_rewrite 1 [←Part.some_get hv]
+    apply Part.eq_map₂_some
+
+  /-- A combinatory algebra is a PCA -/
+  instance isPCA {A : Type} [CA A] : PCA A where
+    K := .some K
+    S := .some S
+    df_K₀ := by trivial
+    df_K₁ := by intros ; trivial
+    eq_K := by intro _ _ hu hv ; simp [CA.eq_app, hu, hv, CA.eq_K]
+    df_S₀ := by trivial
+    df_S₁ := by intros ; trivial
+    df_S₂ := by intros ; trivial
+    eq_S := by intro _ _ _ hu hv hw ; simp [CA.eq_app, hu, hv, hw, CA.eq_S]
+
+  end CA
