PartialCombinatoryAlgebras/PartialCombinatoryAlgebra.lean
@@ -1,0 +1,202 @@
+import Mathlib.Data.Finset.Basic
+import PartialCombinatoryAlgebras.Basic
+
+/-!
+# Partial combinatory algebras
+
+A partial combinatory algebra is a set equipped with a partial binary operation,
+which has the so-called combinators `K` and `S`. We formalize it in two stages.
+
+We first define the class `PartialApplication` which equips a given set `A` with
+a partial binary operation. One might expect such an operation to have type
+`A → A → Part A`, but this leads to complications because it is not composable.
+So instead we specify that a partial operation is a map of type `Part A → Part A → Part A`.
+In other words, we *always* work with partial elements, and separately state that they are
+total as necessary.
+
+(It would be natural to require that the applications be strict, i.e., if the result is defined
+so are its arguments. An early version did so, but the assumption of strictness was never used.)
+
+We then define the class `PCA` (partial combinatory algebra) to be an extension of
+`PartialApplication`. It prescribed combinators `K` and `S` satisfying the usual properties.
+Following our strategy, `K` and `S` are again partial elements on the carrier set,
+with a separate claim that they are total.
+
+-/
+
+/-- The partial combinatory structure on a set `A`. -/
+class PCA (A : Type*) extends PartialApplication A where
+  K : Part A
+  S : Part A
+  df_K₀ : K ⇓
+  df_K₁ : ∀ {u : Part A}, u ⇓ → (K ⬝ u) ⇓
+  df_S₀ : S ⇓
+  df_S₁ : ∀ {u : Part A}, u ⇓ → (S ⬝ u) ⇓
+  df_S₂ : ∀ {u v : Part A}, u ⇓ → v ⇓ → (S ⬝ u ⬝ v) ⇓
+  eq_K : ∀ (u v : Part A), u ⇓ → v ⇓ → (K ⬝ u ⬝ v) = u
+  eq_S : ∀ (u v w : Part A), u ⇓ → v ⇓ → w ⇓ → S ⬝ u ⬝ v ⬝ w = (u ⬝ w) ⬝ (v ⬝ w)
+
+attribute [simp] PCA.df_K₀
+attribute [simp] PCA.df_K₁
+-- attribute [simp] eq_K
+attribute [simp] PCA.df_S₀
+attribute [simp] PCA.df_S₁
+attribute [simp] PCA.df_S₂
+-- attribute [simp] eq_S
+
+/-- Every PCA is inhabited. We pick K as its default element. -/
+instance PCA.inhabited {A : Type*} [PCA A] : Inhabited A where
+  default := K.get df_K₀
+
+/-! `Expr Γ A` is the type of expressions built inductively from
+    constants `K` and `S`, variables in `Γ` (the variable context),
+    the elements of a carrier set `A`, and formal binary application.
+
+    The usual accounts of PCAs typically do not introduce `K` and `S`
+    as separate constants, because a PCA `A` already contains such combinators.
+    However, as we defined the combinators to be partial elements, it is more
+    convenient to have separate primitive constants denoting them.
+    Also, this way `A` need not be an applicative structure.
+-/
+
+namespace PCA
+
+/-- Expressions with variables from context `Γ` and elements from `A`. -/
+inductive Expr (Γ A : Type*) where
+  /-- Formal expression denoting the K combinator -/
+| K : Expr Γ A
+  /-- Formal expression denoting the S combinator -/
+| S : Expr Γ A
+  /-- An element as a formal expression -/
+| elm : A → Expr Γ A
+  /-- A variable as a formal expression -/
+| var : Γ → Expr Γ A
+  /-- Formal expression application -/
+| app : Expr Γ A → Expr Γ A → Expr Γ A
+
+/-- Formal application as a binary operation `·` -/
+instance Expr.hasDot {Γ A : Type*} : HasDot (Expr Γ A) where
+  dot := Expr.app
+
+section
+  universe u v
+  variable {Γ : Type u} [DecidableEq Γ]
+  variable {A : Type v} [PCA A]
+
+  /-- A valuation `η : Γ → A` assigning elements to variables,
+      with the value of `x` overridden to be `a`. -/
+  @[reducible]
+  def override (x : Γ) (a : A) (η : Γ → A) (y : Γ) : A :=
+    if y = x then a else η y
+
+  /-- Evaluate an expression with respect to a given valuation `η`. -/
+  def eval (η : Γ → A): Expr Γ A → Part A
+  | .K => PCA.K
+  | .S => PCA.S
+  | .elm a => .some a
+  | .var x => .some (η x)
+  | .app e₁ e₂ => (eval η e₁) ⬝ (eval η e₂)
+
+  /-- An expression is said to be defined when it is defined at every valuation. -/
+  def defined (e : Expr Γ A) := ∀ (η : Γ → A), (eval η e) ⇓
+
+  /-- The substitution of an element for the extra variable. -/
+  def subst (x : Γ) (a : A) : Expr Γ A → Expr Γ A
+  | .K => .K
+  | .S => .S
+  | .elm b => .elm b
+  | .var y => if y = x then .elm a else .var y
+  | .app e₁ e₂ => (subst x a e₁) ⬝ (subst x a e₂)
+
+  /-- `abstr e` is an expression with one fewer variables than
+      the expression `e`, which works similarly to function
+      abastraction in the λ-calculus. It is at the heart of
+      combinatory completeness. -/
+  def abstr (x : Γ): Expr Γ A → Expr Γ A
+  | .K => .K ⬝ .K
+  | .S => .K ⬝ .S
+  | .elm a => .K ⬝ .elm a
+  | .var y => if y = x then .S ⬝ .K ⬝ .K else .K ⬝ .var y
+  | .app e₁ e₂ => .S ⬝ (abstr x e₁) ⬝ (abstr x e₂)
+
+  /-- An abstraction is defined. -/
+  @[simp]
+  lemma df_abstr (x : Γ) (e : Expr Γ A) : defined (abstr x e) := by
+    intro η
+    induction e
+    case K => simp [eval]
+    case S => simp [eval]
+    case elm => simp [eval]
+    case var y =>
+      cases (decEq y x)
+      case isFalse h => simp [abstr, eval, h]
+      case isTrue h => simp [abstr, eval, h]
+    case app e₁ e₂ ih₁ ih₂ => simp [eval, ih₁, ih₂]
+
+  /-- `eval_abstr e` behaves like abstraction in the extra variable.
+      This is known as *combinatory completeness*. -/
+  lemma eval_abstr (x : Γ) (e : Expr Γ A) (a : A) (η : Γ → A):
+    eval η (abstr x e ⬝ .elm a) = eval (override x a η) e := by
+    induction e
+    case K => simp [eq_K, eval]
+    case S => simp [eq_S, eq_K, eval]
+    case elm => simp [eq_K, eq_S, eval]
+    case var y =>
+      cases (decEq y x)
+      case isFalse h => simp [eq_K, eval, abstr, override, h]
+      case isTrue h => simp [eq_S, eq_K, eval, abstr, override, h]
+    case app e₁ e₂ ih₁ ih₂ =>
+      simp [abstr, eval] at ih₁
+      simp [abstr, eval] at ih₂
+      simp [eq_S, abstr, eval, df_abstr x _ η, ih₁, ih₂]
+
+  /-- Like `eval_abstr` but with the application on the outside of `eval`. -/
+  lemma eval_abstr_app (η : Γ → A) (x : Γ) (e : Expr Γ A) (u : Part A) (hu : u ⇓) :
+    eval η (abstr x e) ⬝ u = eval (override x (u.get hu) η) e := by
+    calc
+     _ = eval η (abstr x e ⬝ .elm (u.get hu)) := by simp [eval]
+     _ = eval (override x (u.get hu) η) e := by apply eval_abstr
+
+  @[simp]
+  lemma eval_override (η : Γ → A) (x : Γ) (a : A) (e : Expr Γ A) :
+    eval (override x a η) e = eval η (subst x a e) := by
+    induction e
+    case K => simp [eval]
+    case S => simp [eval]
+    case elm => simp [eval]
+    case var y =>
+      cases (decEq y x)
+      case isFalse p => simp [eval, subst, p]
+      case isTrue p => simp [eval, subst, p]
+    case app e₁ e₂ ih₁ ih₂ => simp [eval, ih₁, ih₂]
+
+  /-- Compile an expression to a partial element, substituting
+      the default value for any variables occurring in e. -/
+  @[simp]
+  def compile (e : Expr Γ A) : Part A :=
+    eval (fun _ => default) e
+
+  /-- Evaluate an expression under the assumption that it is closed.
+      Return `inl x` if variable `x` is encountered, otherwise `inr u`
+      where `u` is the partial element so obtained. -/
+  def eval_closed : Expr Γ A → Sum Γ (Part A)
+  | .K => return K
+  | .S => return S
+  | .elm a => return (some a)
+  | .var x => .inl x
+  | .app e₁ e₂ =>
+    do
+      let a₁ ← eval_closed e₁ ;
+      let a₂ ← eval_closed e₂ ;
+      return (a₁ ⬝ a₂)
+
+  syntax:20 "≪" term "≫" term:20 : term
+
+  macro_rules
+  | `(≪ $x:term ≫ $a:term) => `(PCA.abstr $x $a)
+
+  syntax "[pca: " term "]" : term
+  macro_rules
+  | `([pca: $e:term ]) => `(PCA.compile (Γ := Lean.Name) $e)
+
+end
